code/ecdsap256/Hacl.Impl.P256.Field.fsti
@@ -15,6 +15,8 @@ module SM = Hacl.Spec.P256.MontgomeryMultiplication
 
 #set-options "--z3rlimit 50 --fuel 0 --ifuel 0"
 
+let fmont_as_nat (h:mem) (a:felem) = SM.fromDomain_ (as_nat h a)
+
 val fmod_short: x:felem -> res:felem -> Stack unit
   (requires fun h ->
     live h x /\ live h res /\ eq_or_disjoint x res)
@@ -29,8 +31,8 @@ val fadd: x:felem -> y:felem -> res:felem -> Stack unit
     eq_or_disjoint x y /\ eq_or_disjoint x res /\ eq_or_disjoint y res /\
     as_nat h x < S.prime /\ as_nat h y < S.prime)
   (ensures  fun h0 _ h1 -> modifies (loc res) h0 h1 /\
-    as_nat h1 res == (as_nat h0 x + as_nat h0 y) % S.prime /\
-    as_nat h1 res == SM.toDomain_ ((SM.fromDomain_ (as_nat h0 x) + SM.fromDomain_ (as_nat h0 y)) % S.prime))
+    as_nat h1 res == S.fadd (as_nat h0 x) (as_nat h0 y) /\
+    fmont_as_nat h1 res == S.fadd (fmont_as_nat h0 x) (fmont_as_nat h0 y))
 
 
 inline_for_extraction noextract
@@ -41,7 +43,7 @@ val fdouble: x:felem -> res:felem -> Stack unit
   (ensures fun h0 _ h1 -> modifies (loc res) h0 h1 /\
     as_nat h1 res == (2 * as_nat h0 x) % S.prime /\
     as_nat h1 res < S.prime /\
-    as_nat h1 res == SM.toDomain_ (2 * SM.fromDomain_ (as_nat h0 x) % S.prime))
+    fmont_as_nat h1 res == (2 * fmont_as_nat h0 x) % S.prime)
 
 
 // NOTE: changed precondition `eq_or_disjoint x y`
@@ -51,8 +53,8 @@ val fsub: x:felem -> y:felem -> res:felem -> Stack unit
     eq_or_disjoint x y /\ eq_or_disjoint x res /\ eq_or_disjoint y res /\
     as_nat h x < S.prime /\ as_nat h y < S.prime)
   (ensures fun h0 _ h1 -> modifies (loc res) h0 h1 /\
-    as_nat h1 res == (as_nat h0 x - as_nat h0 y) % S.prime /\
-    as_nat h1 res == SM.toDomain_ ((SM.fromDomain_ (as_nat h0 x) - SM.fromDomain_ (as_nat h0 y)) % S.prime))
+    as_nat h1 res == S.fsub (as_nat h0 x) (as_nat h0 y) /\
+    fmont_as_nat h1 res == S.fsub (fmont_as_nat h0 x) (fmont_as_nat h0 y))
 
 
 // TODO: rename
@@ -61,7 +63,7 @@ val fromDomain: a:felem -> res:felem -> Stack unit
     live h a /\ live h res /\ as_nat h a < S.prime)
   (ensures  fun h0 _ h1 -> modifies (loc res) h0 h1 /\
     as_nat h1 res = (as_nat h0 a * SM.mont_R_inv) % S.prime /\
-    as_nat h1 res = SM.fromDomain_ (as_nat h0 a))
+    as_nat h1 res = fmont_as_nat h0 a)
 
 
 val fmul: a:felem -> b:felem -> res:felem -> Stack unit
@@ -72,8 +74,7 @@ val fmul: a:felem -> b:felem -> res:felem -> Stack unit
   (ensures fun h0 _ h1 -> modifies (loc res) h0 h1 /\
     as_nat h1 res < S.prime /\
     as_nat h1 res = (as_nat h0 a * as_nat h0 b * SM.mont_R_inv) % S.prime /\
-    as_nat h1 res = SM.toDomain_ (SM.fromDomain_ (as_nat h0 a) * SM.fromDomain_ (as_nat h0 b) % S.prime) /\
-    as_nat h1 res = SM.toDomain_ (SM.fromDomain_ (as_nat h0 a) * SM.fromDomain_ (as_nat h0 b)))
+    fmont_as_nat h1 res = S.fmul (fmont_as_nat h0 a) (fmont_as_nat h0 b))
 
 
 val fsqr: a:felem -> res:felem -> Stack unit
@@ -82,8 +83,7 @@ val fsqr: a:felem -> res:felem -> Stack unit
   (ensures  fun h0 _ h1 -> modifies (loc res) h0 h1 /\
     as_nat h1 res < S.prime /\
     as_nat h1 res = (as_nat h0 a * as_nat h0 a * SM.mont_R_inv) % S.prime /\
-    as_nat h1 res = SM.toDomain_ (SM.fromDomain_ (as_nat h0 a) * SM.fromDomain_ (as_nat h0 a) % S.prime) /\
-    as_nat h1 res = SM.toDomain_ (SM.fromDomain_ (as_nat h0 a) * SM.fromDomain_ (as_nat h0 a)))
+    fmont_as_nat h1 res = S.fmul (fmont_as_nat h0 a) (fmont_as_nat h0 a))
 
 
 ///  Special cases of the above functions
@@ -94,19 +94,8 @@ val fcube: a:felem -> res:felem -> Stack unit
     as_nat h a < S.prime)
   (ensures fun h0 _ h1 -> modifies (loc res) h0 h1 /\
     as_nat h1 res < S.prime /\
-    as_nat h1 res = SM.toDomain_ (SM.fromDomain_ (as_nat h0 a) * SM.fromDomain_ (as_nat h0 a) * SM.fromDomain_ (as_nat h0 a) % S.prime) /\
-    as_nat h1 res = SM.toDomain_ (SM.fromDomain_ (as_nat h0 a) * SM.fromDomain_ (as_nat h0 a) * SM.fromDomain_ (as_nat h0 a)))
-
-
-inline_for_extraction noextract
-val fmul_by_2: a:felem -> res:felem -> Stack unit
-  (requires fun h ->
-    live h a /\ live h res /\ eq_or_disjoint a res /\
-    as_nat h a < S.prime)
-  (ensures fun h0 _ h1 -> modifies (loc res) h0 h1 /\
-    as_nat h1 res == SM.toDomain_ (2 * SM.fromDomain_ (as_nat h0 a) % S.prime) /\
-    as_nat h1 res == SM.toDomain_ (2 * SM.fromDomain_ (as_nat h0 a)) /\
-    as_nat h1 res < S.prime)
+    fmont_as_nat h1 res =
+      S.fmul (S.fmul (fmont_as_nat h0 a) (fmont_as_nat h0 a)) (fmont_as_nat h0 a))
 
 
 val fmul_by_3: a:felem -> res:felem -> Stack unit
@@ -115,8 +104,7 @@ val fmul_by_3: a:felem -> res:felem -> Stack unit
     as_nat h a < S.prime)
   (ensures fun h0 _ h1 -> modifies (loc res) h0 h1 /\
     as_nat h1 res < S.prime /\
-    as_nat h1 res == SM.toDomain_ (3 * SM.fromDomain_ (as_nat h0 a) % S.prime) /\
-    as_nat h1 res == SM.toDomain_ (3 * SM.fromDomain_ (as_nat h0 a)))
+    fmont_as_nat h1 res == (3 * fmont_as_nat h0 a) % S.prime)
 
 
 val fmul_by_4: a:felem -> res:felem -> Stack unit
@@ -125,8 +113,7 @@ val fmul_by_4: a:felem -> res:felem -> Stack unit
     as_nat h a < S.prime)
   (ensures fun h0 _ h1 -> modifies (loc res) h0 h1 /\
     as_nat h1 res < S.prime /\
-    as_nat h1 res == SM.toDomain_ (4 * SM.fromDomain_ (as_nat h0 a) % S.prime) /\
-    as_nat h1 res == SM.toDomain_ (4 * SM.fromDomain_ (as_nat h0 a)))
+    fmont_as_nat h1 res == (4 * fmont_as_nat h0 a) % S.prime)
 
 
 val fmul_by_8: a:felem -> res:felem -> Stack unit
@@ -135,5 +122,4 @@ val fmul_by_8: a:felem -> res:felem -> Stack unit
     as_nat h a < S.prime)
   (ensures fun h0 _ h1 -> modifies (loc res) h0 h1 /\
     as_nat h1 res < S.prime /\
-    as_nat h1 res == SM.toDomain_ (8 * SM.fromDomain_ (as_nat h0 a) % S.prime) /\
-    as_nat h1 res == SM.toDomain_ (8 * SM.fromDomain_ (as_nat h0 a)))
+    fmont_as_nat h1 res == (8 * fmont_as_nat h0 a) % S.prime)
